Add Record wos

wo.v
@@ -1,1 +1,45 @@
-(* The definition of a well-order *)
+(* Well-ordering *)
+
+From set_theory Require Import lib set.
+
+(* Well-Ordering Structure *)
+Record wos (X : Type) := Well_order {
+  prec         : X -> X -> Prop;
+  irreflexive  : ∀x, ¬(prec x x);
+  transitive   : ∀x y z, prec x y -> prec y z -> prec x z;
+  total        : ∀x y, prec x y \/ x = y \/ prec y x;
+  wellorder    : ∀V : P X, V ≠ ∅ -> ∃x, V x /\ ∀y, prec y x -> ¬V y;
+}.
+
+Arguments prec {_}.
+Arguments irreflexive {_}.
+Arguments transitive {_}.
+Arguments total {_}.
+Arguments wellorder {_}.
+
+Notation "x '≺_' A '`' y" := (prec A x y)
+  (at level 30, A at next level, format "x  '≺_' A '`'  y").
+
+(* A progressive property of a well-order is universal. *)
+Theorem wos_ind X (A : wos X) (V : P X) :
+  (∀x, (∀y, y ≺_A` x -> V y) -> V x) -> ∀x, V x.
+Proof.
+(* This is the contra-position of wellorder on the complement of V. *)
+pose(Vneg x := ¬V x); intros HV.
+assert(HVneg : ¬(Vneg ≠ ∅)). {
+  apply (contra _ _ (wellorder A Vneg)).
+  apply all_not_not_ex; intros x [H1x H2x].
+  apply H1x, HV; intros. now apply NNPP, H2x. }
+apply NNPP in HVneg; apply eq_incl in HVneg as [HVneg _].
+intros x; destruct (classic (V x)). easy. now apply HVneg in H.
+Qed.
+
+(* A well-order has no infinite decreasing chains. *)
+Theorem wos_no_infinite_descent X (A : wos X) (f : nat -> X) :
+  ¬∀n, f (S n) ≺_A` f n.
+Proof.
+pose(V x := ∃n, x = f n).
+assert(V ≠ ∅) by (apply not_empty; exists (f 0); now exists 0).
+apply (wellorder A) in H as [x [[n Hn] Hx]]; subst.
+intros H; eapply Hx. apply H. now exists (S n).
+Qed.
